Cleaning Adequacy + weaken the def of state interp. (wip)

theories/weakestpre/adequacy.v
@@ -5,49 +5,242 @@ From iris.proofmode Require Import proofmode.
 From osiris Require Import base.
 From osiris.lang Require Import locations lang.
 From osiris.semantics Require Import semantics.
-From osiris.weakestpre Require Import safe wp.
+From osiris.weakestpre Require Import safe wp helpers.
 
-(* This module proves the adequacy (i.e. the soundness) of our logic. *)
 
-(* ------------------------------------------------------------------------ *)
+Section Adequacy.
+  Context `{!osirisGS_gen Σ}.
 
-(* Boilerplate. *)
+  (* [wp_progress] is an iterated version of [wp_step]. *)
+  Lemma wp_progress n :
+    forall {A σ1 σn} {m1 mn : free A} {s E φ},
+    nsteps step n (σ1, m1) (σn, mn) →
+    state_interp σ1 -∗
+    wp s E m1 φ ={E,∅}=∗
+    |={∅}▷=>^n |={∅,E}=> state_interp σn ∗ wp s E mn φ.
+  Proof.
+    induction n as [ | n IHn] => A σ1 σn m1 mn s E φ /=.
+    { iIntros ([->->]%invert_nsteps_0%pair_equal_spec) "$$".
+      iApply fupd_mask_subseteq; by apply empty_subseteq. }
+    { iIntros (([σm mm]&Hstep&Hsteps)%nsteps_S_inv) "??".
+      iPoseProof ((wp_step Hstep) with "[$][$]") as ">Hstep".
+      iModIntro.
+      iApply ((step_fupdN_wand _ _ 1) with "Hstep").
+      iIntros "H".
+      destruct n.
+      { apply invert_nsteps_0 in Hsteps.
+        simplify_eq/=. done. }
+      { simpl. iMod "H" as "[??]".
+        iPoseProof (IHn _ _ _ _ _ _ _ _ Hsteps) as "IH".
+        by iMod ("IH" with "[$][$]"). } }
+  Qed.
 
-(* It would be nice if someone could explain to me what this means. *)
+End Adequacy.
 
-Class osirisPre Σ := OsirisPre {
+Section Adequacy.
+  Import uPred.
 
-  (* This gives us fancy updates. *)
-  osiris_invGpreS  :> invGpreS Σ;
+  Let inverse_modalities {Σ} `(!invGS_gen HasNoLc Σ) (P : iProp Σ) n :
+    (|={∅}▷=>^n |={∅}=> P) ⊢
+    |={∅}=> |={∅}▷=>^n P.
+  Proof.
+    destruct n.
+    - simpl. by iMod 1.
+    - iIntros"H".
+      by iMod (step_fupdN_S_fupd with "H") as "H".
+  Qed.
 
-  (* This gives us a heap, which maps locations to values. *)
-  osiris_heapGpreS :> gen_heapGpreS loc val Σ;
+  Class required_cmras Σ :=
+    {
+      heap : inG Σ (reservation_map.reservation_mapR (agreeR positiveO)) ;
+      heap' : inG Σ (gmap_view.gmap_viewR loc (leibnizO val)) ;
+      heap'' : inG Σ (gmap_view.gmap_viewR loc (leibnizO gname)) ;
+      wsat_inv : inG Σ (gmap_view.gmap_viewR positive (laterO (iPropO Σ)));
+      wsat_enabled : inG Σ coPset.coPset_disjR;
+      wsat_disabled : inG Σ (gset.gset_disjR positive) ;
+      lc : inG Σ (authR natUR)
+    }.
 
-}.
+  (* These two local lemmas are required in order to recover the requirements of
+     [gen_heap_init] and [step_fupdN_soundness_no_lc]. *)
+  Let required_camras_heap {Σ} :
+    required_cmras Σ → gen_heapGpreS loc val Σ.
+  Proof. intros []; by repeat constructor. Qed.
+  Let required_camras_inv {Σ} :
+    required_cmras Σ → invGpreS Σ.
+  Proof. intros []; by repeat constructor. Qed.
 
-(* This is our closed-world Σ. *)
+  Let wp_pre_adequacy :
+    ∀ {Σ : gFunctors},
+    required_cmras Σ →
+    ∀ {P : iProp Σ} {_: Plain P},
+    ∀ n : nat,
+    (⊢ ∀ `{Hstore: @gen_heapGS loc val Σ loc_eq_decision loc_countable}
+         `{Hinv : invGS_gen HasNoLc Σ},
+       state_interp ∅
+       ={⊤,∅}=∗ |={∅}▷=>^n P)%I →
+    ⊢ P.
+  Proof.
+    iIntros (Σ HΣ P HP n H).
 
-Local Definition osirisΣ : gFunctors :=
-  #[invΣ; gen_heapΣ loc val].
+    (* First, we use an Iris soundness lemma to introduce the required
+       modalities. The soundness lemma will also provide us with a valid [Hinv]
+       to pass to [H]. *)
+    eapply (step_fupdN_soundness_no_lc _ n O).
+    iIntros (Hinv) "_". (* We do not care about later credits. *)
 
-(* These instance declarations are (implicitly) used in the proof of the
-   adequacy lemma that follows. *)
+    (* Now, initialize the heap. *)
+    iPoseProof (@gen_heap_init loc _ _ val Σ _ ∅) as ">(%Hstore&?&_)".
+    iAssert (state_interp ∅) with "[$]" as "?".
 
-Local Instance subG_osirisPre {Σ} :
-  subG osirisΣ Σ -> osirisPre Σ.
-Proof. solve_inG. Qed.
+    (* Use the hypothesis on the provability of [P]. *)
+    iApply (H $! Hstore Hinv with "[$]").
 
-Local Instance osirisPre_osirisΣ : osirisPre osirisΣ.
-Proof. eauto with typeclass_instances. Qed.
+    (* cmras needed to use the heap and invariants are present in Σ. *)
+    Unshelve. all: by eauto.
+  Qed.
 
-(* ------------------------------------------------------------------------ *)
+  Lemma wp_adequacy {A} `{!required_cmras Σ}
+        (s: stuckness) {m1 n σ2 m2} (φ: Prop) :
+    nsteps step n (∅, m1) (σ2, m2) →
+    (⊢ ∀ (Hstore: @gen_heapGS loc val Σ loc_eq_decision loc_countable)
+         (Hinv : invGS_gen HasNoLc Σ),
+       let _ : osirisGS_gen Σ := OsirisG Σ Hinv Hstore in
+       |={⊤}=> ∃ (φ' : A → iProp Σ),
+       wp s ⊤ m1 φ' ∗
+       ( state_interp σ2 -∗
+         wp s ⊤ m2 φ' -∗
+         |={⊤,∅}=> ⌜φ⌝)) →
+    φ.
+  Proof.
+    intros Hsteps H.
 
-(* A first adequacy lemma. *)
+    (* First: setup the iterated later/fupd modalities using the previous local
+              lemma and enter the Iris Proof Mode. *)
+    eapply pure_soundness.
+    eapply (wp_pre_adequacy _ n).
+    iIntros (Hstore Hinv) "Hsi".
 
-Lemma preliminary_adequacy_open
-  {A} Σ `{!osirisPre Σ} s (m : free A) (φ : A → Prop) :
-  (∀ `{!osirisGS_gen Σ}, ⊢ WP m @ s; ⊤ {{ a, ⌜ φ a ⌝ }}) ->
-  safe (∅, m) (λ _ a, φ a).
+    (* Use our hypothesis on the provability of the [wp] and its consequence. *)
+    iMod (H $! Hstore Hinv)  as "(%φ' & ? & Hφ)".
+
+    (* Use preservation of the [wp] and [state_interp] by [n] steps. *)
+    iMod ((wp_progress _ Hsteps) with "[Hsi][$]") as "H".
+    { done. } (* FIXME: replacing [Hsi] by [$] above should work. *)
+
+    (* Inverse some modalities. *)
+    iApply (inverse_modalities Hinv ⌜φ⌝ n).
+
+    (* Use our preservation hypothesis to retrieve the state and [wp]. *)
+    iApply (step_fupdN_wand with "H").
+    iMod 1 as "[? Hwp]".
+
+    (* We have [wp _ _ m2 _] and [state_interm σ2]. Hence, [Hφ] gives us [φ]. *)
+    iApply ("Hφ" with "[$][$]").
+  Qed.
+
+  (* ------------------------------------------------------------------------ *)
+
+  (* The following lemma is a corollary of the adequacy lemma:
+     Let [φ] be a predicate over some type [A].
+     If [wp _ _ m1 (λ v, ⌜φ v⌝)] holds in the Iris logic, and if [(∅, m1)] steps
+        to [(σn, mn)],
+     then [mn] is not stuck, and if it represents a value [v], then [φ v] holds.
+   *)
+  Lemma wp_adequacy' {A} `{!required_cmras Σ}
+        s {m1 n σn mn} (φ : A → Prop) :
+    (* [(∅, m1)] reduces to ([σn, mn)] in n steps. *)
+    nsteps step n (∅, m1) (σn, mn) →
+
+    (* [wp _ _ m1 (λ v, ⌜φ v⌝)] holds *)
+    (⊢ ∀ (Hstore: @gen_heapGS loc val Σ loc_eq_decision loc_countable)
+         (Hinv : invGS_gen HasNoLc Σ),
+       let _ : osirisGS_gen Σ := OsirisG Σ Hinv Hstore in
+       (wp s ⊤ m1 (λ a, ⌜ φ a ⌝))) →
+
+    (* Then, the resulting configuration is not stuck and should [mn] represent
+       a value [v], [φ v] holds. *)
+    (¬ stuck (σn, mn)) ∧ ∀ a, mn = Ret a → φ a.
+  Proof.
+    intros Hsteps H.
+
+    (* First, we define an new pure proposition [φ']. It is equivalent to the
+       conclusion of the lemma. *)
+    let φ' := constr:(match mn with
+              | ret v => φ v
+              | _ => can_step (σn, mn)
+              end) in
+    apply (@apply φ' (¬ stuck (σn, mn) ∧ (∀ a : A, mn = Ret a → φ a))).
+    { intros Hφ.
+      split.
+      { intros ?.
+        destruct mn; eauto using invert_stuck_ret, can_step_not_stuck. }
+      by intros ?->. }
+
+    (* Now that the goal is easier to understand, we use the adequacy lemma.
+       It provides us with the store- and invariants-related hypotheses to use
+       the provability of [wp _ _ m1 (λ v, ⌜φ v⌝)]. *)
+    eapply (wp_adequacy s _ Hsteps).
+    iIntros (Hstore Hinv).
+
+    iExists (λ v, ⌜φ v⌝)%I.
+    iPoseProof (H $! _ _) as "$". iModIntro.
+
+    (* We now have access to the wtate interp and [wp] of the final
+       configuration, which is enough to prove non-stuckness and the
+       postcondition. *)
+    iIntros "?Hwp".
+
+    (* We proceed by case-analysis on [mn]. *)
+    destruct mn; wp_unfold_all.
+    { (* Case: [mn = Ret _]. *)
+      iMod ("Hwp" with "[$]") as ">[_$]".
+      iApply fupd_mask_intro; [ done | by iIntros "_" ]. }
+    all: iMod ("Hwp" with "[$]") as "[%?]"; done.
+  Qed.
+
+(* TODO is this lemma useful? If so, move it to safe.v where it belongs. *)
+
+Lemma prove_initially_safe {A} :
+  ∀ (n: nat) σ {m : free A} {φ : A → Prop},
+  (
+    ∀ (j : nat) σ' m',
+    j ≤ n →
+    steps j (σ, m) (σ', m') →
+    ¬ stuck (σ', m') ∧ ∀ a, m' = Ret a → φ a
+  ) →
+  initially_safe n (σ, m) (λ _ a, φ a).
 Proof.
-  intros Hwp.
-Abort.
+  induction n; intros σ m φ H.
+  { eauto using initially_safe_zero. }
+  triplicity σ m Hm.
+
+  (* Case: [m] is [ret a]. *)
+  { eapply initially_safe_ret.
+    (* The goal is now [φ a]. *)
+    eapply (H O σ (ret a)); eauto with lia steps. }
+
+  (* Case: [(σ, m)] can step. *)
+  { right. split; [ eauto |]. intros (σ', m') Hstep.
+    eapply IHn.
+    intros j σ'' m'' ? Hsteps.
+    eapply (H (S j)); eauto with lia steps. }
+
+  (* Case: [(σ, m)] is stuck. *)
+  { exfalso. eapply (H O); eauto with lia steps. }
+
+Qed.
+
+Lemma prove_safe {A} σ {m : free A} {φ : A → Prop} :
+  (
+    ∀ j σ' m',
+    steps j (σ, m) (σ', m') →
+    ¬ stuck (σ', m') ∧ ∀ a, m' = Ret a → φ a
+  ) →
+  safe (σ, m) (λ _ a, φ a).
+Proof.
+  unfold safe. eauto using prove_initially_safe.
+Qed.
+
+(* TODO where do we go from here? *)
+End Adequacy.
