theories/weakestpre/helpers.v
@@ -1,0 +1,278 @@
+From iris.base_logic.lib Require Import fancy_updates gen_heap.
+From iris.program_logic Require Import adequacy.
+From iris.proofmode Require Import proofmode.
+
+From osiris Require Import base.
+From osiris.lang Require Import locations lang.
+From osiris.semantics Require Import semantics.
+From osiris.weakestpre Require Import safe wp.
+
+(* This tactic is supposed to unfold all occurrences of [wp]. *)
+
+Ltac wp_unfold_all :=
+  rewrite !wp_unfold /wp_pre /=.
+
+(* This tactic unfolds one occurrence of [wp] at the head of the goal. *)
+
+Ltac wp_unfold_head :=
+  iApply wp_unfold; rewrite /wp_pre /=.
+
+(* This tactic unfolds [wp] applied to the computation [m]. *)
+
+Ltac wp_unfold m :=
+  setoid_rewrite (wp_unfold m); rewrite /wp_pre /=.
+
+Section boilerplate.
+
+Context {A : Type}.
+Context `{!osirisGS_gen Σ}.
+Implicit Type s : stuckness.
+Implicit Type P : iProp Σ.
+Implicit Type φ : A → iProp Σ.
+Implicit Type a : A.
+Implicit Type m : free A.
+
+Lemma wp_value_fupd' s E (φ: A -> iProp Σ) m v :
+  (|={E}=> φ v)%I ⊢ WP (Ret v) @ s; E {{ φ }}.
+Proof.
+  iIntros "H".
+  wp_unfold_all.
+  iIntros (?)"$".
+  iMod "H".
+  iMod (@fupd_mask_subseteq _ _ E ∅) as "Hmod"; first set_solver.
+  iModIntro; iMod "Hmod"; iModIntro; iFrame.
+Qed.
+
+Lemma fupd_wp s E m (φ: A -> iProp Σ) :
+  (|={E}=> WP m @ s; E {{ φ }}) ⊢ WP m @ s; E {{ φ }}.
+Proof.
+  iIntros "H".
+  wp_unfold_all.
+  by destruct (is_ret m);
+  iIntros (?)"?";
+  iMod ("H" with "[$]") as "H".
+Qed.
+
+Lemma wp_strong_mono s1 s2 E1 E2 m Φ Ψ :
+  s1 ⊑ s2 → E1 ⊆ E2 →
+  WP m @ s1; E1 {{ Φ }} -∗ (∀ v, Φ v ={E2}=∗ Ψ v) -∗ WP m @ s2; E2 {{ Ψ }}.
+Proof.
+  iIntros (_ HE).
+  iLöb as "IH" forall (m).
+  iIntros "H1 Himpl".
+  wp_unfold_all.
+  iIntros (?)"?". iSpecialize ("H1" with "[$]").
+  iMod (fupd_mask_subseteq E1) as "H"; first assumption.
+  iMod "H1".
+  iModIntro.
+  destruct (is_ret m).
+  { iMod "H1" as "[$?]". iMod "H" as "_".
+    iApply ("Himpl" with "[$]"). }
+  { iDestruct "H1" as "[% H1]".
+    iSplit; first done.
+    iIntros(? m' ?).
+    iSpecialize ("H1" with "[//]").
+    (iMod "H1"; iModIntro).
+    iModIntro.
+    (iMod "H1"; iModIntro).
+    iApply (fupd_trans _ E1).
+    iMod "H1" as "[$H1]".
+    iMod "H" as "_".
+    iPoseProof (@fupd_mask_subseteq _ _ E2 E1) as "H"; first assumption.
+    do 2 (iMod "H"; iModIntro).
+    iApply ("IH" $! m' with "H1 Himpl"). }
+Qed.
+
+Lemma wp_fupd s E m Φ :
+  WP m @ s; E {{ v, |={E}=> Φ v }} ⊢ WP m @ s; E {{ Φ }}.
+Proof.
+  iLöb as "IH" forall (m).
+  iIntros "Hwp".
+  wp_unfold_all.
+  iIntros(σ) "Hsi".
+  iSpecialize ("Hwp" with "Hsi").
+  iMod "Hwp". iModIntro.
+  destruct (is_ret m).
+  { iMod "Hwp" as "[$$]". }
+  { iDestruct "Hwp" as "[%Hcan_step Hwp]". iSplit; first done.
+    iIntros (σ' m' Hstep).
+    iSpecialize ("Hwp" with "[//]").
+    iMod "Hwp".
+    do 2 iModIntro.
+    do 2 (iMod "Hwp"; iModIntro).
+    iDestruct "Hwp" as "[$Hwp]".
+    iApply ("IH" with "Hwp"). }
+Qed.
+
+End boilerplate.
+
+(* -------------------------------------------------------------------------- *)
+
+(* Local tactics. *)
+
+(* [wp_case_is_ret m Hret] performs a case analysis on [m]: either it is
+   of the form [ret a], or it is not. In the second branch, the equality
+   [is_ret m = None] appears under the name [Hret]. *)
+
+Ltac wp_case_is_ret m Hret :=
+  case_eq (is_ret m); [
+    intros ? Hret;
+    apply invert_is_ret_Some in Hret; subst m
+  | intros Hret
+  ].
+
+(* The following tactics corresponds to the branch [is_ret _ = Some _] in
+   the definition of [wp]. This branch is a conjunction
+     state_interp σ ∗ φ v
+   [destruct_wp_ret] is used when this form appears in the hypothesis "Hwp". *)
+
+Ltac destruct_wp_ret :=
+  iMod "Hwp"; iModIntro;
+  iMod "Hwp" as "[Hsi Hwp]"; iModIntro.
+
+(* The following two tactics correspond to the branch [is_ret _ = None] in
+   the definition of [wp]. This branch is a conjunction
+     ⌜can_step (σ, m)⌝ ∗ ∀ σ' m', ...
+   [construct_wp_nonret] is used when this form appears in the goal.
+   [destruct_wp_nonret] is used when it appears in the hypothesis "Hwp". *)
+
+Ltac construct_wp_nonret :=
+  iSplitR; [
+    (* Prove [can_step]: *)
+    iPureIntro; eauto with step can_step
+  | (* Introduce a hypothetical step: *)
+    iIntros (σ' m') "%Hstep"
+  ].
+
+Ltac destruct_wp_nonret :=
+  iMod "Hwp" as "[%Hcanstep Hwp]".
+
+(* Working with the state interpretation invariant. *)
+
+(* [intro_state] introduces [σ] and [state_interp σ]. *)
+(* [spec_state H] specializes the hypothesis H with [state_interp σ]. *)
+(* [release_state] abandons [state_interp σ]. *)
+
+Ltac intro_state :=
+  iIntros (σ) "Hsi".
+
+Ltac spec_state H :=
+  iSpecialize (H with "Hsi").
+
+Ltac release_state :=
+  iFrame "Hsi".
+
+(* [tick_wp] is used when the goal is
+   [|==> ▷ (state_interp σ' ∗ wp E m' φ)]. *)
+
+Ltac tick_wp :=
+  iModIntro; iNext; iMod "Hwp"; iModIntro;
+  iMod "Hwp" as "[$ Hwp]";
+  iModIntro.
+
+(* [step_wp] is used when the hypothesis "Hwp" has the form
+     ∀ σ' m', ⌜step (σ, m) (σ', m')⌝ ==∗ ...
+              ▷ (state_interp σ' ∗ wp E m' φ)
+
+   It applies this hypothesis to a fact of the form [step (σ, m) _],
+   which must appear in the context, and destructs the result. *)
+
+Ltac step_wp :=
+  iMod ("Hwp" with "[//]") as "Hwp".
+
+(* -------------------------------------------------------------------------- *)
+
+(* The following contains low-level reasoning rules of our program logic. *)
+
+(* These rules are applied in [rules.v]. *)
+
+Section rules.
+
+Context `{!osirisGS_gen Σ}.
+
+(* This technical lemma allows grabbing the state invariant when the
+   goal is a [WP] assertion. *)
+
+Lemma wp_grab {A} (m : free A) s E φ :
+  (∀ σ, state_interp σ -∗
+        |={E,∅}=> |={∅,E}=> state_interp σ ∗ WP m @ s; E {{ φ }}
+  ) -∗
+  WP m @ s; E {{ φ }}.
+Proof.
+  iIntros "Hwp". wp_unfold m.
+  intro_state. spec_state "Hwp".
+  iMod "Hwp". iMod "Hwp" as "[Hsi Hwp]".
+  spec_state "Hwp". eauto.
+Qed.
+
+(* -------------------------------------------------------------------------- *)
+
+(* Preservation. *)
+
+(* The assertion [WP m @ s; E {{ φ }}] is preserved by a reduction step. *)
+
+Lemma wp_step {A σ σ'} {m m' : free A} {s E φ} :
+  step (σ, m) (σ', m') →
+  state_interp σ -∗
+  WP m @ s; E {{ φ }} ={E,∅}=∗
+  |={∅}▷=> |={∅,E}=> (
+    state_interp σ' ∗
+    WP m' @ s; E {{ φ }}
+  ).
+Proof.
+  intro Hstep.
+  iIntros "Hsi Hwp".
+  wp_unfold m. spec_state "Hwp".
+  assert (is_not_ret m) as -> by eauto using can_step_is_not_ret with step.
+  destruct_wp_nonret.
+  step_wp.
+  eauto.
+Qed.
+
+(* Progress. *)
+
+Opaque stuck. (* TODO *)
+
+Lemma wp_not_stuck {A} {σ} {m : free A} s E {φ} :
+  state_interp σ -∗
+  WP m @ s; E {{ φ }} -∗
+  |={E,∅}=> ⌜ ¬ stuck (σ, m) ⌝.
+Proof.
+  iIntros "Hsi Hwp".
+  wp_unfold m. spec_state "Hwp".
+  wp_case_is_ret m Hret; [ iMod "Hwp" | destruct_wp_nonret ];
+    iModIntro; iPureIntro.
+  (* Case: [m] is [ret a]. *)
+  (* [ret a] is not stuck. *)
+  { eauto using invert_stuck_ret. }
+  (* Case: [m] can step. *)
+  (* A configuration that can step is not stuck. *)
+  { eauto using can_step_not_stuck. }
+Qed.
+
+(* The following lemma state that given [wp _ m _] and a state interpretation of
+   [σ], the configuration [(σ, m)] can take a step. *)
+Lemma wp_can_step {A σ φ} {m: free A} {s E}:
+  state_interp σ -∗
+  wp s E m φ ={E,∅}=∗ ⌜can_step (σ, m) ∨ is_ret m <> None ⌝.
+Proof.
+  iIntros "? Hwp".
+  wp_unfold_all.
+  iMod ("Hwp" with "[$]") as "Hwp".
+  destruct (is_ret m).
+  { iMod "Hwp". iApply fupd_mask_intro; [ set_solver | iIntros "_" ].
+    iPureIntro. right; by inversion 1. }
+  { iDestruct "Hwp" as "[[%x %Hstep] _]". destruct x as [σ' m'].
+    iModIntro.  eauto with step. }
+Qed.
+
+(* Ditto for a different mask. *)
+Lemma wp_can_step' {A σ φ} {m: free A} {s E}:
+  state_interp σ -∗
+  wp s E m φ ={E}=∗ ⌜can_step (σ, m) ∨ is_ret m <> None ⌝.
+Proof.
+  iIntros "??";
+    iPoseProof (wp_can_step with "[$][$]") as "?".
+  iApply (fupd_plain_mask_empty with "[$]").
+Qed.
+End rules.
